some lemmas about derivative after rotating axis

CartIR.v
@@ -29,7 +29,32 @@ Defined.
 
 Lemma normIRInvSpec : ∀ (pt : Cart2D IR)  (nz : 0 [<] normIR pt), 
    (normIR pt) * (normIRInv pt nz) = 1.
-Admitted.
+  intros. unfold normIRInv. 
+  unfoldMC. unfold Plus_instance_IR, Mult_instance_IR, Zero_instance_IR,
+    Negate_instance_IR.
+  rewrite field_mult_inv.
+  reflexivity.
+Qed.
+
+Lemma MultIRSqrMix: 
+∀ a b : IR, 
+ (a * a * b * b = (a * b) * (a * b)).
+  intros. 
+   unfoldMC. unfold Plus_instance_IR, Mult_instance_IR, Zero_instance_IR,
+    Negate_instance_IR.
+  ring.
+Qed.
+
+Lemma normIRInv2 : ∀ (pt : Cart2D IR)  (nz : 0 [<] normIR pt), 
+   (normSqr pt) * (normIRInv pt nz) * (normIRInv pt nz) = 1.
+  intros. rewrite <- normIRSpec.
+  rewrite MultIRSqrMix.
+  rewrite normIRInvSpec.
+
+  unfoldMC. unfold Plus_instance_IR, Mult_instance_IR, Zero_instance_IR,
+    Negate_instance_IR, One_instance_IR.
+    ring.
+Qed.
 
 (** rotate the axis so that the X axis points
     towards xAxisDir*)
@@ -63,3 +88,61 @@ Proof.
   unfold normIRInv. rewrite field_mult_inv.
   ring.
 Qed.
+
+Lemma rotateOriginTowardsNormSqrPreserved 
+    : ∀ (XTowards : Cart2D IR)
+  (nz : 0 [<] normIR XTowards) pt,
+  normSqr (rotateOriginTowards XTowards nz pt)
+  = normSqr pt.
+Proof.
+  intros. unfold rotateOriginTowards.
+  unfold normSqr. simpl.
+  unfoldMC. unfold Plus_instance_IR, Mult_instance_IR, Zero_instance_IR,
+    Negate_instance_IR.
+  match goal with
+  [ |-_  [=] ?r] => assert (r [=] r [*] [1]) as Heq by ring
+  end.
+  ring_simplify.
+  rewrite <- normIRInv2 with (nz:=nz) in Heq.
+  unfold normSqr in Heq.
+  rewrite Heq.
+  unfoldMC. unfold Plus_instance_IR, Mult_instance_IR, Zero_instance_IR,
+    Negate_instance_IR.
+  ring.
+Qed.
+
+Definition ConstTContR (c : IR) : TContR :=
+  (ContConstFun _ _ c).
+
+Definition rotateOriginTowardsF
+  (XTowards : Cart2D IR)
+  (nz : 0 [<] normIR XTowards)
+  (pt : Cart2D TContR) : Cart2D TContR :=
+  let normInv :=  (normIRInv XTowards nz) in 
+  let Xf := ConstTContR (normInv * X XTowards) in 
+  let Yf := ConstTContR (normInv * Y XTowards) in 
+{|X:= (Xf * X pt + Yf * Y pt);
+  Y:= (Yf * X pt - Xf * Y pt)|}.
+
+Lemma DerivativerotateOriginTowards :
+  ∀ (XTowards : Cart2D IR)
+  (nz : 0 [<] normIR XTowards)
+  (pt : Cart2D TContR) (Dx Dy : TContR),
+  let normInv :=  (normIRInv XTowards nz) in 
+  let Xf := ConstTContR (normInv * X XTowards) in 
+  let Yf := ConstTContR (normInv * Y XTowards) in 
+  let ptR := rotateOriginTowardsF XTowards nz pt in 
+  isDerivativeOf Dx (X pt)
+  → isDerivativeOf Dy (Y pt)
+  → (isDerivativeOf (Xf*Dx + Yf*Dy) (X ptR)
+      × isDerivativeOf (Yf*Dx - Xf*Dy) (Y ptR)).
+Proof.
+  intros ? ? ? ? ?.
+  simpl. intros H1d H2d.
+  split.
+- apply TContRDerivativePlus;
+    apply TContRDerivativeMultConstL; assumption.
+- apply TContRDerivativePlus;[|apply TContRDerivativeOpp];
+    apply TContRDerivativeMultConstL; assumption.
+Qed.
+
